Add basic timing to Lustre and Lustre

theories/Languages/Lustre.v
@@ -57,6 +57,7 @@ Proof.
   f_equal.
   all: assumption.
 Qed.
+
 Definition sig2T_eq_binder := @sig2T_eq _ binder_dec.
 Arguments sig2T_eq_binder {_ _ _ _}.
 
@@ -72,6 +73,7 @@ Lemma const_inv {ty} (x: const ty) :
 Proof using.
   destruct x as [|b|n]; [left; left|left; right|right]; exists eq_refl; [|exists b|exists n]; exact eq_refl.
 Qed.
+
 Lemma const_dec {ty} (x y: const ty) : {x = y} + {x <> y}.
 Proof.
   destruct x.
@@ -92,21 +94,25 @@ Qed.
 Inductive unop: type -> type -> Set :=
   | Uop_not: unop TInt TInt
   | Uop_neg: unop TInt TInt
+  | Uop_pre: unop TInt TInt
 .
 
 Lemma unop_inv {ty tout} (x: unop ty tout) :
   {eq1 : ty = TInt & {eq2 : tout = TInt & x = eq_rect _ (unop _) (eq_rect _ (fun ty => unop ty _) Uop_not _ (eq_sym eq1)) _ (eq_sym eq2)}} +
-  {eq1 : ty = TInt & {eq2 : tout = TInt & x = eq_rect _ (unop _) (eq_rect _ (fun ty => unop ty _) Uop_neg _ (eq_sym eq1)) _ (eq_sym eq2)}}.
+  {eq1 : ty = TInt & {eq2 : tout = TInt & x = eq_rect _ (unop _) (eq_rect _ (fun ty => unop ty _) Uop_neg _ (eq_sym eq1)) _ (eq_sym eq2)}} +
+  {eq1 : ty = TInt & {eq2 : tout = TInt & x = eq_rect _ (unop _) (eq_rect _ (fun ty => unop ty _) Uop_pre _ (eq_sym eq1)) _ (eq_sym eq2)}}
+  .
 Proof using.
-  destruct x; [left|right]; exists eq_refl, eq_refl; exact eq_refl.
+  destruct x; [left|left|right]; [left|right|]; exists eq_refl, eq_refl; exact eq_refl.
 Qed.
+
 Lemma unop_dec {ty tout} (x y: unop ty tout) : {x = y} + {x <> y}.
 Proof.
-  destruct (unop_inv x) as [[eq1 [eq2 ->]]|[eq1 [eq2 ->]]].
-  all: destruct (unop_inv y) as [[-> [-> ->]]|[-> [-> ->]]].
+  destruct (unop_inv x) as [[[eq1 [eq2 ->]]|[eq1 [eq2 ->]]]|[eq1 [eq2 ->]]].
+  all: destruct (unop_inv y) as [[[-> [-> ->]]|[-> [-> ->]]]|[-> [-> ->]]].
   all: rewrite !(Eqdep_dec.UIP_dec type_dec _ eq_refl); cbn.
   all: rewrite !(Eqdep_dec.UIP_dec type_dec _ eq_refl); cbn.
-  1,4: left; reflexivity.
+  1,5,9: left; reflexivity.
   all: right; discriminate.
 Qed.
 
@@ -134,6 +140,9 @@ Inductive binop: type -> type -> type -> Set :=
   | Bop_lt: binop TInt TInt TBool
   | Bop_ge: binop TInt TInt TBool
   | Bop_gt: binop TInt TInt TBool
+
+  (** Timing bop *)
+  | Bop_arrow: binop TInt TInt TInt
 .
 
 Lemma binop_inv {ty1 ty2 tout} (x: binop ty1 ty2 tout) :
@@ -149,9 +158,11 @@ Lemma binop_inv {ty1 ty2 tout} (x: binop ty1 ty2 tout) :
   {eq1 : ty1 = _ & {eq2 : ty2 = _ & {eqo : tout = _ & x = eq_rect _ (binop _ _) (eq_rect _ (fun ty => binop _ ty _) (eq_rect _ (fun ty => binop ty _ _) Bop_le _ (eq_sym eq1)) _ (eq_sym eq2)) _ (eq_sym eqo)}}} +
   {eq1 : ty1 = _ & {eq2 : ty2 = _ & {eqo : tout = _ & x = eq_rect _ (binop _ _) (eq_rect _ (fun ty => binop _ ty _) (eq_rect _ (fun ty => binop ty _ _) Bop_lt _ (eq_sym eq1)) _ (eq_sym eq2)) _ (eq_sym eqo)}}} +
   {eq1 : ty1 = _ & {eq2 : ty2 = _ & {eqo : tout = _ & x = eq_rect _ (binop _ _) (eq_rect _ (fun ty => binop _ ty _) (eq_rect _ (fun ty => binop ty _ _) Bop_ge _ (eq_sym eq1)) _ (eq_sym eq2)) _ (eq_sym eqo)}}} +
-  {eq1 : ty1 = _ & {eq2 : ty2 = _ & {eqo : tout = _ & x = eq_rect _ (binop _ _) (eq_rect _ (fun ty => binop _ ty _) (eq_rect _ (fun ty => binop ty _ _) Bop_gt _ (eq_sym eq1)) _ (eq_sym eq2)) _ (eq_sym eqo)}}}.
+  {eq1 : ty1 = _ & {eq2 : ty2 = _ & {eqo : tout = _ & x = eq_rect _ (binop _ _) (eq_rect _ (fun ty => binop _ ty _) (eq_rect _ (fun ty => binop ty _ _) Bop_gt _ (eq_sym eq1)) _ (eq_sym eq2)) _ (eq_sym eqo)}}} +
+  {eq1 : ty1 = _ & {eq2 : ty2 = _ & {eqo : tout = _ & x = eq_rect _ (binop _ _) (eq_rect _ (fun ty => binop _ ty _) (eq_rect _ (fun ty => binop ty _ _) Bop_arrow _ (eq_sym eq1)) _ (eq_sym eq2)) _ (eq_sym eqo)}}}.
 Proof using.
   destruct x.
+  1-13: left.
   1-12: left.
   1-11: left.
   1-10: left.
@@ -164,7 +175,7 @@ Proof using.
   1-03: left.
   1-02: left.
   1-01: left.
-  2-13: right.
+  2-14: right.
   all: exists eq_refl, eq_refl, eq_refl; exact eq_refl.
 Qed.
 
@@ -174,6 +185,12 @@ Proof.
   repeat destruct H as [ H | [eq1 [eq2 [eq3 ->]]] ].
   1: destruct H as [eq1 [eq2 [eq3 ->]]].
   all: pose proof (binop_inv y) as H.
+  14: destruct H as [f|[-> [-> [-> ->]]]]; [right|left].
+  15: do 3 (rewrite (Eqdep_dec.UIP_dec type_dec _ eq_refl); cbn); reflexivity.
+  1-13: destruct H as [H|[-> [-> [-> f]]]]; [|
+    right; try discriminate; intros <-;
+    repeat (rewrite (Eqdep_dec.UIP_dec type_dec _ eq_refl) in f; cbn in f); try discriminate
+  ].
   13: destruct H as [f|[-> [-> [-> ->]]]]; [right|left].
   14: do 3 (rewrite (Eqdep_dec.UIP_dec type_dec _ eq_refl); cbn); reflexivity.
   1-12: destruct H as [H|[-> [-> [-> f]]]]; [|
@@ -281,6 +298,7 @@ Proof using.
   all: try solve [repeat eexists; exact eq_refl].
   1,2: exists b, eq_refl; exact eq_refl.
 Qed.
+
 Lemma exp_dec {ty} (e1 e2: exp ty) : {e1 = e2} + {e1 <> e2}.
 Proof.
   revert e2.
@@ -365,8 +383,6 @@ Record node := mk_node {
   n_inputs_equations: incl (List.map (fun '((n, ty) as b) => (n, existT exp ty (EInput b))) n_in) n_body;
   n_no_einputs_in_other: Forall (fun '(name, existT _ ty exp) => ~ In name (map fst n_in) -> has_einput exp = false) n_body;
 }.
-
-
 
 Definition node_eq (n1 n2: node) :=
   n_name n1 = n_name n2 /\
